cp in theories. compiles, but new admits due to abstracting types

examples/ghc/theories/CoreSemantics.v
@@ -48,10 +48,10 @@ Definition subst (e₀ : CoreExpr) (n : Id) (e' : CoreExpr) : CoreExpr :=
                                    (if n == n'
                                     then alts
                                     else map (λ '(k, ns, u), (k, ns, if elem n ns then u else subst u)) alts)
-        | Cast e γ         => Cast (subst e) γ
+(*        | Cast e γ         => Cast (subst e) γ
         | Tick tick e      => Tick tick (subst e)
         | Type_ τ          => Type_ τ
-        | Coercion γ       => Coercion γ
+        | Coercion γ       => Coercion γ *)
       end
   in subst e₀.
 
@@ -82,10 +82,10 @@ Definition substs (e₀ : CoreExpr) (ss : list (Id * CoreExpr)) : CoreExpr :=
                                                              then u
                                                              else subst u))
                                             alts)
-        | Cast e γ        => Cast (subst e) γ
+(*         | Cast e γ        => Cast (subst e) γ
         | Tick tick e     => Tick tick (subst e)
         | Type_ τ         => Type_ τ
-        | Coercion γ      => Coercion γ
+        | Coercion γ      => Coercion γ *)
       end
   in subst e₀.
 
@@ -122,8 +122,8 @@ Proof.
   rewrite /subst /substs.
   match goal with |- ?fix_subst e₀ = ?fix_substs e₀ => set subst := fix_subst; set substs := fix_substs end.
   elim/core_induct: e₀ =>
-    [ n' | lit | e₁  e₂ IH₁ IH₂ | n' e IH | [n' e₁ | bs] e₂ IH₁ IH₂ | e n' τ alts IH₁ IH₂
-    | e γ IH | tick e IH | τ | γ ]
+    [ n' | lit | e₁  e₂ IH₁ IH₂ | n' e IH | [n' e₁ | bs] e₂ IH₁ IH₂ | e n' τ alts IH₁ IH₂ ]
+(*     | e γ IH | tick e IH | τ | γ ] *)
     //=.
   - by rewrite Eq_sym; case: (_ == _).
   - by rewrite IH₁ IH₂.
@@ -139,8 +139,8 @@ Proof.
     + elim: ns {IN} => [|n'' ns IHns] //=.
       by rewrite elemC IHns Eq_sym; case: (_ == _).
     + by rewrite (IH₂ _ _ _ IN).
-  - by rewrite IH.
-  - by rewrite IH.
+(*   - by rewrite IH.
+  - by rewrite IH. *)
 Qed.
 
 Definition subst_expr'
@@ -156,12 +156,12 @@ Definition subst_expr'
              end in
        match expr with
        | Core.Mk_Var v => lookupIdSubst (Panic.someSDoc) subst v
-       | Core.Type_ ty => Core.Type_ ty
-       | Core.Coercion co => Core.Coercion co
+(*        | Core.Type_ ty => Core.Type_ ty
+       | Core.Coercion co => Core.Coercion co *)
        | Core.Lit lit => Core.Lit lit
        | Core.App fun_ arg => Core.App (go fun_) (go arg)
-       | Core.Tick tickish e => CoreUtils.mkTick (substTickish subst tickish) (go e)
-       | Core.Cast e co => Core.Cast (go e) co
+(*       | Core.Tick tickish e => CoreUtils.mkTick (substTickish subst tickish) (go e)
+       | Core.Cast e co => Core.Cast (go e) co *)
        | Core.Lam bndr body =>
          let 'pair subst' bndr' := substBndr subst bndr in
          Core.Lam bndr' (subst_expr doc subst' body)
@@ -200,7 +200,7 @@ Proof.
   move_let => /=;
     rewrite /subst; match goal with |- ?fix_subst e = _ => set subst := fix_subst end.
   rewrite /substExpr (*subst_expr_refix*) /subst_expr.
-  elim: e => [n' | lit | e₁ IH₁ e₂ IH₂ | n' e IH | lb e IH | e IH n' τ alts | e IH γ | tick e IH | τ | γ] //=.
+  elim: e => [n' | lit | e₁ IH₁ e₂ IH₂ | n' e IH | lb e IH | e IH n' τ alts (* | e IH γ | tick e IH | τ | γ  *) ] //=.
   - admit.
   - rewrite IH₁ IH₂ //.
     admit.
@@ -209,7 +209,6 @@ Proof.
     admit.
   - admit.
   - admit.
-  - 
 Abort.
 
 Notation "e @[ n ↦ e' ]" := (subst e n e') (at level 15, no associativity, format "e @[ n  ↦  e' ]").
