examples/ghc/lib/CoreTidy.v
@@ -143,12 +143,8 @@ Definition tidyBind
              end in
            match arg_0__, arg_1__ with
            | env, Core.Mk_Var v => Core.Mk_Var (tidyVarOcc env v)
-           | env => Core.Type_ (TyCoRep.tidyType env ty)
-           | env => Core.Coercion (TyCoRep.tidyCo env co)
            | _, Core.Lit lit => Core.Lit lit
            | env, Core.App f a => Core.App (tidyExpr env f) (tidyExpr env a)
-           | env => Core.Tick (tidyTickish env t) (tidyExpr env e)
-           | env => Core.Cast (tidyExpr env e) (TyCoRep.tidyCo env co)
            | env, Core.Let b e =>
                tidyBind env b =: (fun '(pair env' b') => Core.Let b' (tidyExpr env' e))
            | env, Core.Case e b ty alts =>
@@ -182,12 +178,8 @@ Definition tidyExpr : Core.TidyEnv -> Core.CoreExpr -> Core.CoreExpr :=
              end in
            match arg_0__, arg_1__ with
            | env, Core.Mk_Var v => Core.Mk_Var (tidyVarOcc env v)
-           | env => Core.Type_ (TyCoRep.tidyType env ty)
-           | env => Core.Coercion (TyCoRep.tidyCo env co)
            | _, Core.Lit lit => Core.Lit lit
            | env, Core.App f a => Core.App (tidyExpr env f) (tidyExpr env a)
-           | env => Core.Tick (tidyTickish env t) (tidyExpr env e)
-           | env => Core.Cast (tidyExpr env e) (TyCoRep.tidyCo env co)
            | env, Core.Let b e =>
                tidyBind env b =: (fun '(pair env' b') => Core.Let b' (tidyExpr env' e))
            | env, Core.Case e b ty alts =>
@@ -224,19 +216,17 @@ Infix "CoreTidy.=:" := (_=:_) (at level 99).
 End Notations.
 
 (* External variables:
-     None Some bool co e list op_zt__ pair snd t tt ty Core.App Core.Breakpoint
-     Core.Case Core.Cast Core.Coercion Core.CoreAlt Core.CoreBind Core.CoreExpr
-     Core.Id Core.Lam Core.Let Core.Lit Core.Mk_Var Core.NonRec Core.Rec Core.Tick
-     Core.Tickish Core.TidyEnv Core.Type_ Core.Unfolding Core.Var Core.demandInfo
-     Core.extendVarEnv Core.idDetails Core.idInfo Core.inlinePragInfo
-     Core.isStableUnfolding Core.isTyCoVar Core.lookupVarEnv Core.mkLocalVar
-     Core.noUnfolding Core.occInfo Core.oneShotInfo Core.setArityInfo
+     None Some bool list op_zt__ pair snd tt Core.App Core.Breakpoint Core.Case
+     Core.CoreAlt Core.CoreBind Core.CoreExpr Core.Id Core.Lam Core.Let Core.Lit
+     Core.Mk_Var Core.NonRec Core.Rec Core.Tickish Core.TidyEnv Core.Unfolding
+     Core.Var Core.demandInfo Core.extendVarEnv Core.idDetails Core.idInfo
+     Core.inlinePragInfo Core.isStableUnfolding Core.isTyCoVar Core.lookupVarEnv
+     Core.mkLocalVar Core.noUnfolding Core.occInfo Core.oneShotInfo Core.setArityInfo
      Core.setDemandInfo Core.setInlinePragInfo Core.setOccInfo Core.setOneShotInfo
      Core.setStrictnessInfo Core.setUnfoldingInfo Core.strictnessInfo
      Core.unfoldingInfo Core.vanillaIdInfo Core.zapUsageEnvSig CoreArity.exprArity
      Data.Traversable.mapAccumL GHC.Base.map GHC.Err.default GHC.List.zip
      GHC.Prim.seq Id.idName Id.idType Id.idUnique Id.mkLocalIdWithInfo Maybes.orElse
      Name.Name Name.getOccName Name.mkInternalName OccName.tidyOccName
-     SrcLoc.noSrcSpan TyCoRep.tidyCo TyCoRep.tidyTyCoVarBndr TyCoRep.tidyType
-     UniqFM.lookupUFM
+     SrcLoc.noSrcSpan TyCoRep.tidyTyCoVarBndr TyCoRep.tidyType UniqFM.lookupUFM
 *)
