examples/ghc/theories/ScopeInvariant.v
@@ -126,10 +126,10 @@ Fixpoint WellScoped (e : CoreExpr) (in_scope : VarSet) {struct e} : Prop :=
       Forall GoodLocalVar (snd (fst alt)) /\
       let in_scope' := extendVarSetList in_scope (bndr :: snd (fst alt)) in
       WellScoped (snd alt) in_scope') alts
-  | Cast e _ =>   WellScoped e in_scope
+(*  | Cast e _ =>   WellScoped e in_scope
   | Tick _ e =>   WellScoped e in_scope (* /\ WellScopedTickish t in_scope *)
   | Type_ _  =>   True
-  | Coercion _ => True
+  | Coercion _ => True *)
   end
 with WellScopedBind (bind : CoreBind) (in_scope : VarSet) : Prop :=
   match bind with
@@ -184,10 +184,9 @@ Lemma GoodLocalVar_asJoinId_mkSysLocal:
 Proof.
   move=> s u ty n h1.
   unfold mkSysLocal.
-  split; only 1: split.
-  * destruct u. symmetry.  
 Admitted.
-(*
+(*   split; only 1: split.
+  * destruct u. symmetry.  
     apply h1.
   * split. destruct u. reflexivity. 
     auto.
@@ -205,8 +204,8 @@ Proof.
   destruct H. destruct H.
   induction H0.
   * split; only 1: split; assumption.
-  * split; only 1: split; assumption.
-  * split; only 1: split; assumption.
+(*   * split; only 1: split; assumption.
+  * split; only 1: split; assumption. *)
 Qed.
 
 Lemma GoodVar_almostEqual : 
@@ -247,8 +246,8 @@ Proof.
   intros.
   destruct v; simpl; try trivial.
   unfold varToCoreExpr; simpl.
-  rewrite andb_false_r.
-  destruct_match; simpl; try trivial.
+  rewrite andb_false_r; try done.
+(*  destruct_match; simpl; try trivial. *)
 Qed.
 
 
@@ -470,7 +469,7 @@ Proof.
       apply subVarSet_delVarSetList_extendVarSetList_dual.
       apply (H0 _ _ _ HIn).
       assumption.
-  - rewrite exprFreeVars_Cast. apply H; assumption.
+(*  - rewrite exprFreeVars_Cast. apply H; assumption.
   - rewrite exprFreeVars_Tick.
     simpl in H0.
     by apply H.
@@ -502,7 +501,7 @@ Proof.
     rewrite h in WSy. done.
     *)
   - apply subVarSet_emptyVarSet.
-  - apply subVarSet_emptyVarSet.
+  - apply subVarSet_emptyVarSet. *)
 Qed.
 
 
@@ -709,7 +708,7 @@ Proof.
         epose proof (mapUnionVarSet_In_subVarSet f HIn) as H ; simpl in H end.
       rewrite -> delVarSetList_rev, <- delVarSetList_single, <- delVarSetList_app.
       set_b_iff; fsetdec.
-  * apply H. 
+(*  * apply H. 
     eapply disjointVarSet_subVarSet_l; only 1: apply H0.
     apply subVarSet_delVarSetList_both.
     rewrite exprFreeVars_Cast.
@@ -752,7 +751,7 @@ Proof.
           apply subVarSet_emptyVarSet.
     *)
   * reflexivity.
-  * reflexivity.
+  * reflexivity. *)
 Qed.
 
 Lemma WellScoped_extendVarSetList_fresh:
@@ -860,7 +859,7 @@ Proof.
        specialize (H0 _ _ _ HIn).
        apply Respects_StrongSubset_extendVarSetList.
        apply H0.
-   * apply H.
+(*   * apply H.
    * apply H.
      (*
      unfold Respects_StrongSubset
@@ -871,5 +870,5 @@ Proof.
      eapply Respects_StrongSubset_WellScopedTickish; eauto.
      *)
    * apply Respects_StrongSubset_const.
-   * apply Respects_StrongSubset_const.
+   * apply Respects_StrongSubset_const. *)
 Qed.
